\documentclass{ximera}

\input{../../preamble.tex}

\author{Kenneth Berglund}
\acknowledgement{}

\begin{document}
\licenseSZ
\begin{exercise}
\begin{enumerate}
\item If $f(x) = x^3 - 3$, then $f^{-1}(x) = \answer{\sqrt[3]{x + 3}}$.

\item If $f(x) = \frac{x - 2}{3} + 4$, then $f^{-1}(x) = \answer{3(x - 4) + 2}$.

\item If $f(x) = \frac{3}{4 - x}$, then $f^{-1}(x) = \answer{\frac{4x - 3}{x}}$. 

\item If $f(x) = 1- \frac{4 + 3x}{5}$, then $f^{-1}(x) = \answer{-\frac{5}{3}x + \frac{1}{3}}$.

\item If $f(x) = 3(x + 4)^2 - 5$ for $x \le -4$, then $f^{-1}(x) = \answer{-\sqrt{\frac{x + 5}{3}} - 4}$.

\item If $f(x) = 3(x + 4)^2 - 5$ for $x \ge -4$, then $f^{-1}(x) = \answer{\sqrt{\frac{x + 5}{3}} - 4}$.
\end{enumerate}
\end{exercise}
\end{document}