\documentclass{ximera}

\input{../../preamble.tex}

\author{Kenneth Berglund}
\acknowledgement{}

\begin{document}
In this exercise, we will solve the equation $3^{2x} - 3^x - 6 = 0$.
\begin{exercise}
Notice that $3^{2x}$ is the square of $\answer{3^x}$. If we call $3^x = u$, then $3^{2x} = u^2$. 

\begin{exercise}
Consider the expression $u^2 - u - 6$. This factors as $(u - \answer{3})(u + \answer{2})$. 

\begin{exercise}
The previous factorization and the fact that $(3^x)^2 = 3^{2x}$ allows us to say $3^{2x} - 3^x - 6$ factors as $(3^x - \answer{3})(3^{x} + \answer{2})$. 


\begin{exercise}
Recall that $(3^x - 3)(3^{x} + 2) = 0$ if and only if $3^x - 3 = 0$ or $3^x + 2 = 0$. Therefore, the equation $(3^x - 3)(3^{x} + 2) = 0$ has $\answer{1}$ solution(s).

\begin{exercise}
The solution to $3^{2x} - 3^x - 6 = 0$ is $\answer{1}$.
\end{exercise}
\end{exercise}
\end{exercise}
\end{exercise}


\end{exercise}
\end{document}