\documentclass[nooutcomes]{ximera}

\input{../preamble}
\author{Ivo Terek}
\license{Creative Commons Attribution-ShareAlike 4.0 International License}
\acknowledgement{}

\title{Finding Inverses Algebraically}

\begin{document}
\licenseSZ
\begin{abstract}
  
\end{abstract}
\maketitle


%\typeout{************************************************}
%\typeout{Motivating Questions}
%\typeout{************************************************}

%\begin{motivatingQuestions}\begin{itemize}
%\item What are inverse functions?
%\end{itemize}\end{motivatingQuestions}


%\typeout{************************************************}
%\typeout{Introduction}
%\typeout{************************************************}
In this section, we will practice how to actually algebraically determine whether the inverse for a given function $f$ exists, and how to find it.

\begin{example}
  Let $f$ be the function given by $f(x) = 4x^3+1$, for every real number $x$. Is $f$ one-to-one? If so, what is the inverse $f^{-1}$? What is its domain?

  \begin{explanation}
    Recall here that $f$ is one-to-one if $f(x_1) = f(x_2)$ always implies that $x_1=x_2$. What happens in this case? We start with the equality $$4x_1^3+1 = 4x_2^3+1,$$ and if we can arrive at $x_1=x_2$, then our function $f$ is one-to-one. Subtracting $1$ from both sides gives $4x_1^3=4x_2^3$. Dividing both sides by $4$, we have that $x_1^3 = x_2^3$. As the function ``taking the third power'' is one-to-one (namely, its inverse is ``taking cube roots''), it follows that $x_1=x_2$. This means that one can start with $y=4x^3+1$ and solve for $x$ as a function of $y$. When this is finished, one replaces $x$ and $y$ with $f^{-1}(x)$ and $x$, respectively, for the sake of conventions. We have that $$y=4x^3+1 \implies y-1 = 4x^3 \implies \frac{y-1}{4} = x^3 \implies \sqrt[3]{\frac{y-1}{4}} = x.$$Therefore, we conclude that $$f^{-1}(x) = \sqrt[3]{\frac{x-1}{4}}.$$Observe that the domain of $f^{-1}$ is precisely the set of all real numbers, as there is no positivity restriction for taking ``odd roots''. This turns out to be exactly the range of the original function $f$, suitably read in the $y$ variable: namely, the range of $f$ consists of all real numbers $y$, as the graph shows:
\begin{image}
\begin{tikzpicture}
    \begin{axis}
      \addplot[samples=200,domain=-5:5]{4*x^3+1};
    \end{axis}
\end{tikzpicture}
\end{image}
Observe that the graph also shows that $f$ passes the Horizontal Line Test, a useful sanity check.
  \end{explanation}
\end{example}

\begin{callout}
  What happened with the domain of $f^{-1}$ on the previous example is a very general phenomenon: if a given function $f$ is one-to-one, so that $f^{-1}$ exists, the domain of $f^{-1}$ is exactly the range of the original function $f$.
\end{callout}

\begin{exploration}
   Study the function $f(x) = -x^5 + 10$. Is it one-to-one? If yes, find a formula for $f^{-1}$.
\end{exploration}


\begin{example} 
  Let $g$ be the rational function given by $g(x) = 2x/(1-x)$ for every real number $x$ not equal to $1$. Is $g$ one-to-one? If so, what is the inverse $g^{-1}$? What is its domain?

  \begin{explanation}
    The formula defining $g$ is different from the formula defining the function from the previous example: there, we had a polynomial, while here we have a rational function. The process to study it, however, is the same. To decide whether $g$ is one-to-one or not, we will start with $g(x_1)=g(x_2)$, and try to conclude that $x_1=x_2$. So, we start with $$\frac{2x_1}{1-x_1} = \frac{2x_2}{1-x_2}.$$By cross multiplying, we have that $$2x_1(1-x_2) = 2x_2(1-x_1).$$Distributing the products on both sides, we obtain $$2x_1-2x_1x_2 = 2x_2-2x_2x_1.$$Since $2x_2x_1=2x_1x_2$, adding this quantity to both sides gives us that $2x_1=2x_2$. Finally, dividing everything through by $2$, it follows that $x_1=x_2$. Therefore, $g$ is one-to-one. With this in place, we can attempt to find $g^{-1}$. Starting with $$y = \frac{2x}{1-x},$$the only thing it seems we might be able to try is to cross multiply terms, and distribute the products. So $$(1-x)y = 2x \implies x-xy = 2x.$$As our goal is to solve for $x$ in terms of $y$, let's move everything that contains $x$ in it to one side, and leave the rest which does not contain it on the other side. We obtain $y = 2x+xy$. Factoring $x$, it follows that $y = (2+y)x$. Finally, we conclude that $$x=\frac{y}{y+2}\implies g^{-1}(x) = \frac{x}{x+2},$$by replacing $x$ and $y$ with $g^{-1}(x)$ and $x$, respectively. We observe that the domain of $g^{-1}$ consists of all real numbers $x$ different from $-2$, in the same way that the range of $g$ consists of all real numbers $y$ different from $-2$ (to wit, if we had $-2 = 2x/(1-x)$, then cross multiplying and simplifying yields $-x=1-x$, leading to a terribly nonsensical $0=1$).
  \end{explanation}
\end{example}

\begin{exploration}
  Study the function $g(x) = 3x/(4-5x)$. Is it one-to-one? If yes, find a formula for $g^{-1}$.
\end{exploration}

\begin{example}
  Let $h$ be the function given by $h(x) = e^{\sqrt{x-3}}$ for every real number $x$ greater or equal to $3$. Is $h$ one-to-one? If so, what is the inverse $h^{-1}$? What is its domain?

  \begin{explanation}
    Let's start verifying whether $h$ is one-to-one or not. So, as before, we start with $h(x_1)=h(x_2)$ and try to obtain that $x_1=x_2$. In other words, we start with $e^{\sqrt{x_1-3}} = e^{\sqrt{x_2-3}}$. From arguing either that the exponential function itself is one-to-one, or applying $\ln$ on both sides of this equality, it follows that $\sqrt{x_1-3}=\sqrt{x_2-3}$. Raising both sides to the square, we have that $x_1-3=x_2-3$, and adding $3$ to everything yields $x_1=x_2$, as desired. Therefore, $h$ is one-to-one. To find a formula for $h^{-1}$, we start with $y= e^{\sqrt{x-3}}$ and solve for $x$ in terms of $y$. First, we apply $\ln$ on both sides of the equality, as to obtain $\ln y = \sqrt{x-3}$. Next, we take squares on both sides, so $(\ln y)^2 = x-3$. Finally, we add $3$ to both sides: $$x = (\ln y)^2+3 \implies h^{-1}(x) = (\ln x)^2+3.$$Note that $(\ln x)^2$ is not the same thing as $\ln(x^2)$ (to wit, the latter equals $2\ln x$, by properties of the logarithm function we shall soon see). The inverse $h^{-1}$ is defined for all $x>0$, due to the presence of $\ln x$ in its formula.
  \end{explanation}
\end{example}

\begin{exploration}
  Study the function $h(x) = \ln \sqrt{x+10}$. Is it one-to-one? If yes, find a formula for $h^{-1}$.
\end{exploration}


\end{document}
