
\documentclass{ximera}

\input{../../preamble.tex}

\author{David Kish}
\license{Creative Commons Attribution-ShareAlike 4.0 International License}



\begin{document}
\begin{callout}
  Let $x\geq 0$, $y,m,n >0$, then \\

 \textbf{Product Rule:}
\[ x^{\frac{1}{n}} \cdot x^{\frac{1}{m}} = x^{\frac{1}{n} + \frac{1}{m}}
\]
  %
  \textbf{Power to a Power Rule:}
  \[ \big(x^{\frac{1}{n}}\big)^m = x^{\frac{m}{n}} \]
   \textbf{Product to a Power Rule:}
    \[\big(x \cdot y \big)^{\frac{1}{n}} = x^{\frac{1}{n}} \cdot y^{\frac{1}{n}}
\]
    %
    \textbf{Quotient to a Power Rule:}
  \[\left(\frac{x}{y}\right)^{\frac{1}{n}} = \frac{x^{\frac{1}{n}}}{y^{\frac{1}{n}}} \]
  %
 \textbf{Negative Exponents:}
  \[\frac{x^{\frac{1}{n}}}{x^{\frac{2}{n}}} = \frac{1}{x^{\frac{1}{n}}} = x^{-\frac{1}{n}}\]
\end{callout}
\begin{exercise}
Simplify the expression.\\
\[
\frac{x^5}{x^2}=x^{\answer{3}}
\]
\end{exercise}
\begin{exercise}
Simplify the expression.\\
\[
\frac{x}{x^3}=x^{\answer{-2}}
\]
\end{exercise}
\begin{exercise}
Simplify the expression.\\
\[
x^2\cdot x^7=x^{\answer{9}}
\]
\end{exercise}
\end{document}