\documentclass{ximera}

\input{../../preamble.tex}

\author{Kenneth Berglund}
\acknowledgement{}

\begin{document}
\begin{exercise}
\begin{enumerate}
\item Let $f$ be a function defined by $f(x) = e^x -1$.

The function $f$ has $\answer{1}$ zero(s).

\item Let $g$ be a function defined by $g(x) = e^x + 1$.

The function $g$ has $\answer{0}$ zero(s).

\item Let $h$ be a function defined by $h(x) = x^3 - 4x^2 - x + 4$. \\
  \begin{hint}
   Use the factor-by-grouping method.
  \end{hint}

The function $g$ has $\answer{3}$ zero(s).
\end{enumerate}

\begin{exercise}
\begin{enumerate}
\item Let $f$ be a function defined by $f(x) = e^x -1$.

$f(x)=0$ when $x=\answer {0}$.

\item Let $g$ be a function defined by $g(x) = e^x + 1$.

The function $g$ has no zero(s).

\item Let $h$ be a function defined by $h(x) = x^3 - 4x^2 - x + 4$. \\
  \begin{hint}
   Use the factor-by-grouping method.
  \end{hint}

Give the roots of $h(x)$ in increasing order.

Smallest root: $x=\answer{-1}$ \\
Middle root: $x=\answer{1}$\\
Largest root: $x=\answer{4}$
\end{enumerate}

\end{exercise}

\end{exercise}
\end{document}